Foundation/Propositional/Kripke/AxiomLEM.lean
@@ -12,7 +12,7 @@ section definability
 
 variable {F : Kripke.Frame}
 
-lemma validate_LEM_of_symmetric : Symmetric F → F ⊧ (Axioms.LEM (.atom 0)) := by
+lemma validate_LEM_of_symmetric' : Symmetric F → F ⊧ (Axioms.LEM (.atom 0)) := by
   unfold Symmetric Axioms.LEM;
   contrapose;
   push_neg;
@@ -33,8 +33,9 @@ lemma validate_LEM_of_symmetric : Symmetric F → F ⊧ (Axioms.LEM (.atom 0)) :
   . by_contra Ryx;
     exact h₁ $ Satisfies.formula_hereditary Ryx hy;
 
-lemma validate_LEM_of_euclidean (hEuc : Euclidean F) : F ⊧ (Axioms.LEM (.atom 0)) :=
-  validate_LEM_of_symmetric (symm_of_refl_eucl (by simp [Reflexive, Frame.refl]) hEuc)
+lemma validate_LEM_of_euclidean [IsEuclidean _ F] : F ⊧ (Axioms.LEM (.atom 0)) := by
+  apply validate_LEM_of_symmetric';
+  exact IsSymm.symm;
 
 lemma euclidean_of_validate_LEM : F ⊧ (Axioms.LEM (.atom 0)) → Euclidean F := by
   rintro h x y z Rxy Rxz;
@@ -68,7 +69,7 @@ open Classical
 
 namespace Canonical
 
-protected lemma euclidean [Entailment.HasAxiomLEM 𝓢] : Euclidean (canonicalFrame 𝓢).Rel := by
+instance [Entailment.HasAxiomLEM 𝓢] : IsEuclidean _ (canonicalFrame 𝓢).Rel := ⟨by
   rintro x y z;
   simp [canonicalFrame];
   intro Rxy;
@@ -82,6 +83,7 @@ protected lemma euclidean [Entailment.HasAxiomLEM 𝓢] : Euclidean (canonicalFr
     have : φ ∈ y.1.1:= Rxy $ (or_iff_not_imp_right.mp $ iff_mem₁_or.mp $ mem₁_of_provable (by simp)) hnφ;
     contradiction;
   . exact not_mem₁_neg_of_mem₁ hzφ;
+⟩
 
 end Canonical
 
